

Calcul algébrique

$$x \neq 0$$

$$\begin{aligned} & \bullet (21x^3 - 14x^2 + 7x) : (-7x) - (x-1) \cdot (x+2) = \\ & = \frac{\cancel{7x}^1 (3x^2 - 2x + 1)}{\cancel{-7x}_1} - (x^2 + 2x - x - 2) = \\ & = -3x^2 + 2x - 1 - (x^2 + x - 2) = -3x^2 + 2x - 1 - x^2 - x + 2 = \\ & = \underline{-4x^2 + x + 1} \end{aligned}$$

$$\begin{aligned} & \bullet (x-2) \cdot [4(x+5) - 3(x+6)] - x \cdot (x-4) = \\ & = (x-2) \cdot (4x+20-3x-18) - x^2 + 4x = \\ & = (x-2) \cdot (x+2) - x^2 + 4x = \cancel{x^2} - 4 - \cancel{x^2} + 4x = 4x - 4 \end{aligned}$$

$$\begin{aligned} & \bullet 2 \cdot \left(\frac{\sqrt{7}}{\sqrt{7}-\sqrt{5}} \cdot x \cdot \frac{\sqrt{5}}{\sqrt{7}-\sqrt{5}} \cdot x \right) + \left[(2x-9)^9 \right]' : \left[(9-2x)^7 \right]' = \\ & \text{condition } 9-2x \neq 0 \Leftrightarrow 9 \neq 2x \Leftrightarrow x \neq 9/2 \end{aligned}$$

$$\begin{aligned} & = \frac{2 \cdot \sqrt{35} \cdot x^2}{(\sqrt{7}-\sqrt{5})^2} + (2x-9)^{36} : (9-2x)^{35} = \\ & = \frac{2\sqrt{35}x^2}{(\sqrt{7})^2 - 2\sqrt{7}\sqrt{5} + (\sqrt{5})^2} + (2x-9)^{36} : [-1 \cdot (-9+2x)]^{35} = \end{aligned}$$

$$\begin{aligned} & = \frac{2\sqrt{35}x^2}{12 - 2\sqrt{35}} + (2x-9)^{36} : \left[-(2x-9)^{35} \right] = \\ & = \frac{\cancel{2}\sqrt{35} \cdot x^2}{\cancel{2} \cdot (6 - \sqrt{35})} - (2x-9)^{36-35} = \end{aligned}$$

$$6 + \sqrt{35}$$

$$= \frac{\sqrt{35}x^2}{6 - \sqrt{35}} - 2x + 9 = \frac{6\sqrt{35}x^2 + 35x^2}{6^2 - (\sqrt{35})^2} - 2x + 9 =$$

$$= \frac{(6\sqrt{35} + 35)x^2}{36 - 35} - 2x + 9 = (6\sqrt{35} + 35)x^2 - 2x + 9$$

$$\frac{7 + \sqrt{3}}{7 - \sqrt{3}} \cdot x^2 + 3 \cdot \left[\frac{7 + \sqrt{3}}{7 - \sqrt{3}} \cdot x^2 + 3 \cdot (1 - x) \right] - 3x =$$

$$= \frac{7 + \sqrt{3}}{49 - 3} \cdot x^2 + 3 \cdot \left(\frac{7 + \sqrt{3}}{49 - 3} \cdot x^2 + 3 - 3x \right) - 3x =$$

$$= \frac{(7 + \sqrt{3})}{46} \cdot x^2 + 3 \cdot \frac{(7 + \sqrt{3})x^2}{46} + 9 - 9x - 3x =$$

$$= \frac{(7 + \sqrt{3})}{23} \cdot x^2 - 12x + 9 = \frac{14 + 7\sqrt{3}}{23} \cdot x^2 - 12x + 9$$

$$\left[(3y - x)^{m+3} - (3y - x)^{m+2} \right] : (3y - x) - (3y - x - 1) =$$

$$(in\ condition\ 3y - x \neq 0 \Leftrightarrow 3y \neq x \Leftrightarrow y \neq \frac{x}{3})$$

$$= \frac{(3y - x)^1 \cdot (3y - x)^{m+2} - (3y - x)^{m+2} \cdot 1}{(3y - x)^{m+2}} - 3y + x + 1 =$$

$$= \frac{\cancel{(3y - x)^{m+2}}^1 \cdot (3y - x - 1)}{\cancel{(3y - x)^{m+2}}_1} - 3y + x + 1 =$$

$$= 3y - x - 1 - 3y + x + 1 = 0$$

$$\begin{aligned} & (4a - 2b + 5)^{133} + (-4a + 2b - 5)^{133} = \\ & = (4a - 2b + 5)^{133} + [(-1) \cdot (4a - 2b + 5)]^{133} = \\ & = (4a - 2b + 5)^{133} + (-1) \cdot (4a - 2b + 5)^{133} = \\ & = (4a - 2b + 5)^{133} - (4a - 2b + 5)^{133} = 0 \end{aligned}$$

$$\begin{aligned} & (3x + 7)^2 - (4x - 5)^2 - (7x + 2) \cdot (7x - 2) = \\ & = (3x)^2 + 2 \cdot 3x \cdot 7 + 7^2 - (16x^2 - 40x + 25) - (49x^2 - 4) = \\ & = \underline{9x^2 + 42x + 49} - \underline{16x^2 + 40x - 25} - \underline{49x^2 + 4} = \\ & = -56x^2 + 82x + 28 \end{aligned}$$

$$\left. \begin{aligned} x^2 + y^2 + z^2 &= 216 \\ xy + yz + zx &= 230 \end{aligned} \right\} \Rightarrow \begin{cases} (x+y+z)^2 = x^2 + y^2 + z^2 + 2xy + 2xz + 2yz \\ (x+y+z)^2 = 216 + 2 \cdot 230 = 676 \\ \Rightarrow x+y+z = \pm 26 \end{cases}$$

$$\begin{array}{r|l} 2xy + yz + zx = 230 \cdot 2 & \\ 2xy + 2yz + 2xz = 460 & \\ x^2 + y^2 + z^2 = 216 & \\ \hline & + \end{array}$$

$$\begin{array}{r} \sqrt{676} \quad \left| \begin{array}{l} 26 \\ 46 \cdot 6 = 276 \\ 276 \\ 276 \\ \hline - - - \end{array} \right. \end{array}$$

$$x^2 + y^2 + z^2 + 2xy + 2yz + 2xz = 676 \Rightarrow$$

$$(x+y+z)^2 = 676 \Rightarrow \sqrt{(x+y+z)^2} = \sqrt{676} \Leftrightarrow$$

$$|x+y+z| = 26 \Rightarrow x+y+z = 26 \text{ atau}$$

$$x+y+z = -26$$